Adds comment on the problems of defining Requires as an operation

newio/Free.fst
@@ -6,6 +6,23 @@ type op_sig (op:Type u#a) = {
   res : (cmd:op) -> (args cmd) -> Type u#a;
 }
 
+(** We should try to define PartialCall as an operation, not as a new constructor
+    on the free monad.
+
+    CA: I tried to do this, but there are some universe problems:
+    1. When trying to use add_sig on io_sig and req_sig, I get an error that one signature is
+       u#0 u#0 and the other is u#1 u#0.
+    2. To define an effect, the representation must be polymorphic in exact two universes.
+
+    Some code that may be useful:
+type cmds = | Requires | Openfile | Read | Close | GetTrace
+let _req_cmds (x:cmds) : bool = x = Requires
+type req_cmds : Type0 = x:cmds{_req_cmds x} 
+unfold let req_args (x:req_cmds) : Type u#1 = pure_pre 
+unfold let req_res (x:req_cmds) (pre:req_args x) : Type u#0 = squash pre
+let req_sig : op_sig req_cmds = { args = req_args; res = req_res; }
+**)
+
 noeq
 type free (op:Type0) (s:op_sig op) (a:Type) : Type =
 | Call : (l:op) -> (arg:s.args l) -> cont:(s.res l arg -> free op s a) -> free op s a
